updated it_sems_alt.v

proofs/itrees/it_sems_alt.v
@@ -63,6 +63,7 @@ Definition err_result {E: Type -> Type} `{ErrEvent -< E}
 
 End Errors.
 
+
 (**** JASMIN SEMANTICS *******************************************)
 Section WSW.
 Context
@@ -102,17 +103,18 @@ Definition eval_syscall
 Definition mk_error_data (s:estate) (e:error) : error_data := (e, tt).
 
 (* build our state-sensitive errors *)
-Definition mk_errtype := fun s => mk_error_data s ErrType.
+Definition mk_errtype : estate -> error_data :=
+  fun s => mk_error_data s ErrType.
 
 (*** lifting instruction to itrees *)
-
-Definition iget_fundef {E} `{ErrEvent -< E}
-    (fn: funname) (s:estate) : itree E fundef :=
-  ioget (mk_errtype s) (get_fundef (p_funcs pr) fn).
 
 Definition iresult {E} `{ErrEvent -< E} {T} (s:estate) (F : exec T) :
     itree E T :=
   err_result (mk_error_data s) F.
+
+Definition iget_fundef {E} `{ErrEvent -< E}
+    (fn: funname) (s:estate) : itree E fundef :=
+  ioget (mk_errtype s) (get_fundef (p_funcs pr) fn).
 
 Definition iwrite_var {E} `{ErrEvent -< E}
     (wdb : bool) (x : var_i) (v : value) (s : estate) : itree E estate :=
@@ -137,31 +139,27 @@ Definition isem_pexprs {E} `{ErrEvent -< E}
   iresult s (sem_pexprs wdb gd s es).
 
 (* Auxiliary functions for recursion on list (seq) *)
-Fixpoint isem_map {E} (sem_i: instr_r -> estate -> itree E estate)
+Fixpoint isem_ir_map {E} (R: instr_r -> estate -> itree E estate)
    (c: cmd) (st: estate) : itree E estate :=
   match c with
   | nil => Ret st
-  | (MkI _ i) :: c' => st' <- sem_i i st ;; isem_map sem_i c' st'
+  | (MkI _ i) :: c' => st' <- R i st ;; isem_ir_map R c' st'
   end.
 
-
-(**********************************************************************)
-(*** error-aware interpreter with mutual recursion *)
+Fixpoint isem_i_map {E} (R: instr -> estate -> itree E estate)
+   (c: cmd) (st: estate) : itree E estate :=
+  match c with
+  | nil => Ret st
+  | i :: c' => st' <- R i st ;; isem_i_map R c' st'
+  end.
 
 (* function call info record *)
 Record fstate := mk_fstate
       { fscs : syscall_state_t; fmem : mem; fvals : values }.
-(*
-Record fc_info : Type := mk_fc_info {
-  fc_scs : syscall_state_t ;
-  fc_m : mem ;
-  fc_vs : values }.                           
-*)
 
-(* mutual recursion events *)
-Variant MREvent : Type -> Type :=
- | LCode (c: cmd) (st: estate) : MREvent estate
- | FCall (f: funname) (fc: fstate) : MREvent fstate.
+(**********************************************************************)
+(*** error-aware interpreter with mutual recursion *)
+
 
 Notation it_continue_loop st := (ret (inl st)).
 Notation it_exit_loop st := (ret (inr st)).
@@ -175,7 +173,239 @@ Definition isem_bound {E} `{ErrEvent -< E} (e:pexpr) (s: estate) :
     itree E Z :=
   iresult s (sem_pexpr true pglobs s e >>r= to_int).
 
+Section REC_sem.
+
 Fixpoint isem_for_body {E} `{ErrEvent -< E}
+   (RL : instr -> estate -> itree E estate)
+   (i: var_i) (c: cmd)
+   (ls: list Z) (s: estate) : itree E estate :=
+  match ls with
+  | nil => ret s
+  | (w :: ws) =>
+    s <- iwrite_var true i (Vint w) s;;
+    s <- isem_i_map RL c s;;
+    isem_for_body RL i c ws s
+  end.
+  
+Definition isem_while_body {E} `{ErrEvent -< E}
+   (RC : instr -> estate -> itree E estate)
+   (c1 : cmd) (e:pexpr) (c2: cmd) (s1 : estate) : itree E (estate + estate) :=
+   s2 <- isem_i_map RC c1 s1 ;;
+   b <- isem_cond e s2 ;;
+   if b then s3 <- isem_i_map RC c2 s2 ;; it_continue_loop s3
+   else it_exit_loop s2.
+
+Definition isem_while {E} `{ErrEvent -< E}
+   (RC : instr -> estate -> itree E estate)
+   (c1 : cmd) (e:pexpr) (c2: cmd) (s1 : estate) : itree E estate :=
+  ITree.iter (isem_while_body RC c1 e c2) s1.
+
+Definition isem_call {E} `{ErrEvent -< E}
+    (RC: funname -> fstate -> itree E fstate)                  
+    (xs: lvals) (fn: funname) (args: pexprs) (s1: estate) :
+    itree E estate :=
+  vargs <- isem_pexprs  (~~direct_call) pglobs s1 args ;;
+  r <- RC fn (mk_fstate (escs s1) (emem s1) vargs) ;;
+  iwrite_lvals (~~direct_call) pglobs
+       (with_scs (with_mem s1 r.(fmem)) r.(fscs)) xs r.(fvals).
+
+(* isem_i_body *)
+Fixpoint isem_instrF {E} `{ErrEvent -< E}
+   (RC : funname -> fstate -> itree E fstate)
+   (i: instr) (s1: estate) : itree E estate :=
+  let sem_i := isem_instrF RC in
+  let sem_cmd := isem_i_map sem_i in
+  let: (MkI _ i) := i in
+  match i with
+  | Cassgn x tg ty e => iresult s1 (eval_assgn x tg ty e s1)
+  | Copn xs tg o es => iresult s1 (sem_sopn pglobs o s1 xs es)
+  | Csyscall xs o es => iresult s1 (eval_syscall xs o es s1)
+
+  | Cif e c1 c2 =>
+    b <- isem_cond e s1;;
+    sem_cmd (if b then c1 else c2) s1
+
+  | Cwhile a c1 e c2 =>
+    isem_while sem_i c1 e c2 s1
+
+  | Cfor i (d, lo, hi) c =>
+    vlo <- isem_bound lo s1 ;;
+    vhi <- isem_bound hi s1 ;;
+    isem_for_body sem_i i c (wrange d vlo vhi) s1
+
+  | Ccall xs fn args => isem_call RC xs fn args s1
+  end.                                
+
+Definition estate0 (fs : fstate) :=
+  Estate fs.(fscs) fs.(fmem) Vm.init.
+
+Definition initialize_fcall (fd:fundef) (fs:fstate) : exec estate :=
+  let sinit := estate0 fs in
+  Let vargs' := mapM2 ErrType dc_truncate_val fd.(f_tyin) fs.(fvals) in
+  Let s0 := init_state fd.(f_extra) (p_extra pr) ev sinit in
+  write_vars (~~direct_call) fd.(f_params) vargs' s0.
+
+Definition finalize_fcall (fd : fundef) (s:estate) :=
+  Let vres := get_var_is (~~ direct_call) s.(evm) fd.(f_res) in
+  Let vres' := mapM2 ErrType dc_truncate_val fd.(f_tyout) vres in
+  let scs := s.(escs) in
+  let m := finalize fd.(f_extra) s.(emem) in
+  ok {| fscs := scs; fmem := m; fvals := vres' |}.
+
+Definition isem_fcall_bodyF {E} `{ErrEvent -< E}
+   (RC : funname -> fstate -> itree E fstate)
+   (fn : funname) (fs:fstate) : itree E fstate :=
+  (* FIXME: this is durty : sinit*)
+  let sinit := estate0 fs in
+  fd <- iget_fundef fn sinit;;
+  s1 <- iresult sinit (initialize_fcall fd fs);;
+  s2 <- isem_i_map (isem_instrF RC) fd.(f_body) s1;;
+  iresult s2 (finalize_fcall fd s2).
+
+Notation CALL := (callE (funname * fstate) fstate).
+
+(* rec_call *)
+Definition trigger_call {E}
+    (fn: funname) (fc: fstate) : itree (CALL +' E) fstate :=
+  trigger (Call (fn, fc)).
+
+(* isem_i_rec *)
+Definition isem_instr {E} `{ErrEvent -< E} (i : instr) (s1: estate) : itree (CALL +' E) estate :=
+  isem_instrF trigger_call i s1.
+
+Definition isem_cmd {E} `{ErrEvent -< E} (c : cmd) (s : estate) :
+  itree (CALL +' E) estate :=
+  isem_i_map isem_instr c s.
+
+(* isem_call_rec *)
+Definition isem_fcall_body {E} `{ErrEvent -< E} :                       
+   funname -> fstate -> itree (CALL +' E) fstate :=
+  isem_fcall_bodyF trigger_call .
+
+Definition isem_fcall_body' {E} `{ErrEvent -< E} (x: funname * fstate) : itree (CALL +' E) fstate :=
+  isem_fcall_body (fst x) (snd x).
+
+(* interp_recCall *)
+Definition handle_fcall {E} `{ErrEvent -< E} : CALL ~> itree (CALL +' E) :=
+  calling' isem_fcall_body'.
+
+(* isem_call *)
+Definition isem_fcall {E} `{ErrEvent -< E}
+   (fn : funname) (fs : fstate) : itree E fstate :=
+  rec isem_fcall_body' (fn, fs).
+
+(* isem_i *)
+Definition isem_flat_instr {E} `{ErrEvent -< E} (i : instr) (s : estate) :
+  itree E estate :=
+  isem_instrF isem_fcall i s.
+
+(* isem_cmd *)
+Definition isem_flat_cmd {E} `{ErrEvent -< E} (c : cmd) (s : estate) :
+  itree E estate :=
+  isem_i_map isem_flat_instr c s.
+
+(* sem_call *)
+Definition final_isem_call (fn : funname) (fs : fstate) :
+  execT (itree void1) (fstate) :=
+  interp_Err (isem_fcall fn fs).
+
+Lemma interp_ioget {E : Type -> Type} `{ErrEvent -< E} Err T (o : option T) :
+  eutt (E:=E) eq (interp (mrecursive (D:=CALL) handle_fcall) (ioget Err o))
+                 (ioget Err o).
+Proof.
+  case o => /=.
+  + move=> ?; rewrite interp_ret; reflexivity.
+  rewrite interp_vis bind_trigger.
+  by apply eqit_Vis => -[].
+Qed.
+
+Lemma interp_iresult {E : Type -> Type} `{ErrEvent -< E} s T (r : exec T) :
+  eutt (E:=E) eq (interp (mrecursive (D:=CALL) handle_fcall) (iresult s r)) (iresult s r).
+Proof.
+  case r => /=.
+  + move=> ?; rewrite interp_ret; reflexivity.
+  move=> e; rewrite interp_vis bind_trigger.
+  by apply eqit_Vis => -[].
+Qed.
+
+Lemma interp_isem_cmd {E} `{ErrEvent -< E} c s :
+  eutt (E:=E) eq
+    (interp (mrecursive handle_fcall) (isem_cmd c s))
+    (isem_flat_cmd c s).
+Proof.
+  apply: (cmd_rect
+    (Pr := fun ir => forall ii s,
+               eutt (E:=E) eq (interp (mrecursive handle_fcall) (isem_instr (MkI ii ir) s))
+                              (isem_flat_instr (MkI ii ir) s))
+    (Pi := fun i => forall s,
+       eutt (E:=E) eq (interp (mrecursive handle_fcall) (isem_instr i s))
+                      (isem_flat_instr i s))
+    (Pc := fun c => forall s,
+       eutt (E:=E) eq (interp (mrecursive handle_fcall) (isem_cmd c s))
+                      (isem_flat_cmd c s))) c s => //=.
+  + move=> s; rewrite interp_ret; reflexivity.
+  + move=> i c hi hc s; rewrite interp_bind;apply eqit_bind; first by apply hi.
+    by move=> s'; apply hc.
+  + intros.
+    by move=> >; apply interp_iresult.
+  + by move=> >; apply interp_iresult.
+  + by move=> >; apply interp_iresult.
+  + move=> e c1 c2 hc1 hc2 ii s; rewrite /isem_instr /isem_flat_instr /=.
+    rewrite interp_bind; apply eqit_bind.
+    + by apply interp_iresult.
+    by move=> []; [apply hc1 | apply hc2].
+  + move=> v dir lo hi c hc ii s; rewrite /isem_instr /isem_flat_instr /=.
+    rewrite interp_bind; apply eqit_bind; first by apply interp_iresult.
+    move=> vlo.
+    rewrite interp_bind; apply eqit_bind; first by apply interp_iresult.
+    move=> vhi; elim: wrange s => {vlo vhi ii} //=.
+    + move=> >; rewrite interp_ret; reflexivity.
+    move=> j js hrec s.
+    rewrite interp_bind; apply eqit_bind; first by apply interp_iresult.
+    move=> s'; rewrite interp_bind.
+    rewrite hc; setoid_rewrite hrec; reflexivity.
+  + move=> al c1 e c2 hc1 hc2 ii s; rewrite /isem_instr /isem_flat_instr /= /isem_while.
+    rewrite interp_iter; apply eutt_iter => {}s.
+    rewrite /isem_while_body.
+    rewrite interp_bind; apply eqit_bind; first by apply hc1.
+    move=> s1; rewrite interp_bind; apply eqit_bind; first by apply interp_iresult.
+    move=> [].
+    + rewrite interp_bind; apply eqit_bind; first by apply hc2.
+      move=> s2; rewrite interp_ret; reflexivity.
+    rewrite interp_ret; reflexivity.
+  move=> xs f es ii s; rewrite /isem_instr /isem_flat_instr /=.
+  rewrite interp_bind; apply eqit_bind; first by apply interp_iresult.
+  move=> vs.
+  rewrite interp_bind; apply eqit_bind; last by move=> >; apply interp_iresult.
+  rewrite interp_mrecursive; reflexivity.
+Qed.
+  
+End REC_sem.
+
+
+Section MREC_sem.
+
+(*
+Definition jsem_while_body {E} `{ErrEvent -< E}
+   (RL : instr_r -> estate -> itree E estate)
+   (c1 : cmd) (e:pexpr) (c2: cmd) (s1 : estate) : itree E (estate + estate) :=
+   s2 <- isem_ir_map RL c1 s1 ;;
+   b <- isem_cond e s2 ;;
+   if b then s3 <- isem_ir_map RL c2 s2 ;; it_continue_loop s3
+   else it_exit_loop s2.
+
+Definition jsem_while {E} `{ErrEvent -< E}
+   (RL : instr_r -> estate -> itree E estate)
+   (c1 : cmd) (e:pexpr) (c2: cmd) (s1 : estate) : itree E estate :=
+  ITree.iter (jsem_while_body RL c1 e c2) s1.
+*)  
+
+(* mutual recursion events *)
+Variant MREvent : Type -> Type :=
+ | LCode (c: cmd) (st: estate) : MREvent estate
+ | FCall (f: funname) (fc: fstate) : MREvent fstate.
+
+Fixpoint jsem_for_body {E} `{ErrEvent -< E}
    (RL : cmd -> estate -> itree E estate)
    (i: var_i) (c: cmd) (ls: list Z) (s: estate) : itree E estate :=
   match ls with
@@ -183,29 +413,21 @@ Fixpoint isem_for_body {E} `{ErrEvent -< E}
   | (w :: ws) =>
     s <- iwrite_var true i (Vint w) s;;
     s <- RL c s;;
-    isem_for_body RL i c ws s
+    jsem_for_body RL i c ws s
   end.
 
-Definition isem_while_body {E} `{ErrEvent -< E}
-    (RL : cmd -> estate -> itree (MREvent +' E) estate)
+Definition jsem_while_body {E} `{ErrEvent -< E}
+    (RL : cmd -> estate -> itree E estate)
     (c1 c2: cmd) (e: pexpr) (s1: estate) :
-    itree (MREvent +' E) (estate + estate) :=
+    itree E (estate + estate) :=
   s2 <- RL c1 s1 ;; 
   b <- isem_cond e s2 ;; 
   if b then s3 <- RL c2 s2 ;; it_continue_loop s3 
   else it_exit_loop s2. 
 
-Definition isem_call {E} `{ErrEvent -< E}
-    (RC: funname -> fstate -> itree  (MREvent +' E) fstate)                  
-    (xs: lvals) (fn: funname) (args: pexprs) (s1: estate) :
-    itree (MREvent +' E) estate :=
-  vargs <- isem_pexprs  (~~direct_call) pglobs s1 args ;;
-  res <- it_rec_call (FCall fn (mk_fstate (escs s1) (emem s1) vargs)) ;;
-  iwrite_lvals (~~direct_call) pglobs
-       (with_scs (with_mem s1 res.(fmem)) res.(fscs)) xs res.(fvals).
-  
+
 (* instruction semantic functor *)
-Definition isem_instrF {E} `{ErrEvent -< E}
+Definition jsem_instrF {E} `{ErrEvent -< E}
   (RL : cmd -> estate -> itree (MREvent +' E) estate)
   (RC: funname -> fstate -> itree  (MREvent +' E) fstate)
     (i : instr_r) (s1: estate) :
@@ -218,27 +440,27 @@ Definition isem_instrF {E} `{ErrEvent -< E}
       b <- isem_cond e s1;;
       RL (if b then c1 else c2) s1
   | Cwhile a c1 e c2 =>
-      ITree.iter (isem_while_body RL c1 c2 e) s1
+      ITree.iter (jsem_while_body RL c1 c2 e) s1
   | Cfor i (d, lo, hi) c =>
      vlo <- isem_bound lo s1 ;;
      vhi <- isem_bound hi s1 ;;
-     isem_for_body RL i c (wrange d vlo vhi) s1
+     jsem_for_body RL i c (wrange d vlo vhi) s1
   | Ccall xs fn args => isem_call RC xs fn args s1 
 end.
 
-Definition isem_fcall {E} `{ErrEvent -< E} 
+Definition jsem_fcall {E} `{ErrEvent -< E} 
     (fn: funname) (fc: fstate) : itree (MREvent +' E) fstate :=
   it_rec_call (FCall fn fc).
 
 (* event-based recursion *)
 Definition msem_instr {E} `{ErrEvent -< E}
     (i : instr_r) (s1: estate) : itree (MREvent +' E) estate :=
-  isem_instrF (fun c s => it_rec_call (LCode c s)) isem_fcall i s1.
+  jsem_instrF (fun c s => it_rec_call (LCode c s)) isem_fcall i s1.
 
 (* fixpoint-based recursion *)
 Fixpoint rsem_instr {E} `{ErrEvent -< E}
     (i : instr_r) (s1: estate) : itree (MREvent +' E) estate :=
-  isem_instrF (isem_map rsem_instr) isem_fcall i s1.
+  jsem_instrF (isem_ir_map rsem_instr) isem_fcall i s1.
 
 Definition initialize_call (scs1 : syscall_state_t) (m1 : mem)
     (fd : fundef) (vargs : values) : exec estate :=
@@ -254,22 +476,22 @@ Definition finalize_call (fd : fundef) (s:estate) :=
   let m := finalize fd.(f_extra) s.(emem) in
   ok (mk_fstate scs m vres').
 
-Definition sem_call_body {E} `{ErrEvent -< E}
-   (fn : funname) (fc: fstate) : itree (MREvent +' E) fstate :=
+Definition jsem_call_body {E} `{ErrEvent -< E}
+   (fn : funname) (fs: fstate) : itree (MREvent +' E) fstate :=
   (* FIXME: this is durty : sinit*)
-  let sinit := (Estate fc.(fscs) fc.(fmem) Vm.init) in
+  let sinit := estate0 fs in
   fd <- iget_fundef fn sinit;;
-  s1 <- iresult sinit (initialize_call fc.(fscs) fc.(fmem) fd fc.(fvals));;
+  s1 <- iresult sinit (initialize_fcall fd fs);;
   s2 <- it_rec_call (LCode fd.(f_body) s1);;
-  iresult s2 (finalize_call fd s2).
+  iresult s2 (finalize_fcall fd s2).
 
 Definition sem_mreventF {E} `{ErrEvent -< E}
    (R : instr_r -> estate -> itree (MREvent +' E) estate) :
    MREvent ~> itree (MREvent +' E) :=
  fun _ fs =>
    match fs with
-   | LCode c st => isem_map R c st
-   | FCall fn fc => sem_call_body fn fc
+   | LCode c st => isem_ir_map R c st
+   | FCall fn fc => jsem_call_body fn fc
    end.
 
 Definition sem_callF {E} `{ErrEvent -< E}
@@ -299,15 +521,7 @@ Definition final_rsem_call (fn : funname) (fc: fstate) :
     execT (itree void1) fstate :=
   interp_Err (rsem_call fn fc).
 
-(******************************************************************)
-
-Variant RecCode : Type -> Type :=
- | RECCode (c: cmd) (st: estate) : RecCode estate.
-
-Variant RecCall : Type -> Type :=
-  | RECCall (fn: funname) (fc: fstate) : RecCall fstate.
-
-Definition FCState : Type -> Type := (RecCode +' RecCall).
+End MREC_sem.
 
 End WSW.
 
